bottom up approach

Affine/Lambda.lean
@@ -13,12 +13,21 @@ inductive Lambda : Type
 
 namespace Lambda
 
-/-- The size of a lambda, useful for `termination_by`. -/
+/-- The depth of a lambda, useful for `termination_by`. -/
 def depth (e : Lambda) : ℕ :=
   match e with
   | .var _ => 0
   | .abs _ e => 1 + e.depth
   | .app e₁ e₂ => 1 + max e₁.depth e₂.depth
+
+/-- The number of β-reductions. That is, `(λ x. e₁) e₂`. -/
+def count_β (e : Lambda) : ℕ :=
+  match e with
+  | .var _ => 0
+  | .abs _ e => e.count_β
+  | .app (.var _) e₂ => e₂.count_β
+  | .app (.abs _ e₁) e₂ => 1 + e₁.count_β + e₂.count_β
+  | .app (.app e₁ e₂) e₃ => e₁.count_β + e₂.count_β + e₃.count_β
 
 /-- Number of times `x` occurs freely in `e`. -/
 def count (e : Lambda) (x : ℕ) : ℕ :=
@@ -39,7 +48,7 @@ def is_affine (e : Lambda) : Bool :=
   match e with
   | .var _ => true
   | .abs x e => is_affine e ∧ e.count x ≤ 1
-  | .app e₁ e₂ => is_affine e₁ ∧ is_affine e₂ ∧ ∀ x ∈ e.free, e₁.count x + e₂.count x ≤ 1
+  | .app e₁ e₂ => is_affine e₁ ∧ is_affine e₂ ∧ e₁.free ∩ e₂.free = ∅
 
 def to_string (e : Lambda) : String :=
   match e with
