Affine/Normalize.lean
@@ -1,170 +1,109 @@
-import «Affine».Lemmas
+import «Affine».Conversion
+import «Affine».Substitution
 import «Affine».Misc
 
 namespace Lambda
 
-/-- Replaces free occurrences of variable `x` with variable `y`. -/
-def substᵥ (e : Lambda) (x y : ℕ) : Lambda :=
-  match e with
-  | .var x' => if x = x' then .var y else .var x'
-  | .app e₁ e₂ => .app (e₁.substᵥ x y) (e₂.substᵥ x y)
-  | .abs x' e => if x = x' then .abs x' e else .abs x' (e.substᵥ x y)
-
-/-- Variable substitution preserves depth. Needed for `termination_by` in `substₑ`. -/
-@[simp] theorem substᵥ_depth_eq (e : Lambda) (x y : ℕ) : (e.substᵥ x y).depth = e.depth := by
-  match e with
-  | .var x' => simp only [substᵥ, depth, apply_ite, ite_self]
-  | .app e₁ e₂ => simp only [substᵥ, depth, substᵥ_depth_eq]
-  | .abs x' e => simp only [substᵥ, apply_ite, depth, substᵥ_depth_eq, ite_self]
-
-/-- Substitutes free occurrences of variable `x` in `e₁` with `e₂`. -/
-def substₑ (e₁ : Lambda) (x : ℕ) (e₂ : Lambda) : Lambda :=
-  match e₁ with
-  | .var x' => if x = x' then e₂ else e₁
-  | .app a₁ a₂ => .app (a₁.substₑ x e₂) (a₂.substₑ x e₂)
-  | .abs x' e₁ =>
-    if x = x' ∨ x ∉ e₁.free then
-      .abs x' e₁
-    else if x' ∈ e₂.free then
-      let y := e₂.free.fresh
-      .abs y ((e₁.substᵥ x' y).substₑ x e₂)
-    else
-      .abs x' (e₁.substₑ x e₂)
-termination_by e₁.depth
-
-@[simp] theorem substₑ_count_mem_free (e₁ e₂ : Lambda) (hx : x ∈ e₁.free) :
-    (e₁.substₑ x e₂).count y = (e₁.count x) * (e₂.count y) := by
-  match e₁ with
-  | .var x' => simp only [substₑ, if_pos (Finset.mem_singleton.mp hx), count, one_mul]
-  | .abs x' e₁ =>
-    have hx : ¬(x = x' ∨ x ∉ e₁.free) := by
-      simp_rw [not_or, not_not, ← Finset.mem_singleton.not, and_comm, ← Finset.mem_sdiff]
-      exact hx
-
-    simp only [substₑ, if_neg hx_ne]
-
-
-@[simp] theorem substₑ_of_not_mem_free (e₁ e₂ : Lambda) (h : x ∉ e₁.free) :
-    e₁.substₑ x e₂ = e₁ := by
-  match e₁ with
-  | .var x' => simp only [substₑ, if_neg (Finset.mem_singleton.not.mp h)]
-  | .abs x' e₁ =>
-    simp only [free, Finset.mem_sdiff, not_and_or, not_not] at h
-    by_cases hx : x = x'
-    · simp only [substₑ, if_pos (Or.inl hx)]
-    · have : x ∉ e₁.free := by simp only [Finset.mem_singleton, hx, or_false] at h; exact h
-      simp only [substₑ, if_pos (Or.inr this)]
-  | .app a₁ a₂ =>
-    simp only [free, Finset.not_mem_union] at h
-    simp only [substₑ, substₑ_of_not_mem_free a₁ e₂ h.left, substₑ_of_not_mem_free a₂ e₂ h.right]
-
-@[simp] theorem substₑ_count_not_mem_free (e₁ e₂ : Lambda) (h : x ∉ e₁.free) :
-    (e₁.substₑ x e₂).count y = e₁.count y := by
-  simp only [substₑ_of_not_mem_free e₁ e₂ h]
-
-@[simp] theorem substₑ_count_mem_free_of_affine
-    (e₁ e₂ : Lambda) (h : x ∈ e₁.free) (he₁ : e₁.is_affine) :
-    (e₁.substₑ x e₂).count y = e₁.count y := by
-  simp only [substₑ_of_not_mem_free e₁ e₂ h]
-
-theorem substₑ_free_eq (e₁ e₂ : Lambda) (x : ℕ) :
-    (e₁.substₑ x e₂).free = e₁.free \ {x} ∪ e₂.free := by
-  sorry
-
--- theorem substₑ_count_affine_le {e₁ e₂ : Lambda} : (e₁.substₑ y e₂).count y = e₂.count y := by
---   match e₁ with
---   | .var x' =>
---     simp only [substₑ, apply_ite (count · y)]
---     by_cases hx : y = x'
---     · simp only [hx, ↓reduceIte]
---     · simp [hx, count]
-
--- theorem substₑ_count_ne_eq {e₁ e₂ : Lambda} (h : x ≠ y) : (e₁.substₑ x e₂).count y = e₁.count x + e₂.count x := by sorry
-
-
-/-- Substitution of affine terms preserves top-level affinity (free variable count at most one). -/
--- theorem substₑ_count_le {e₁ e₂ : Lambda} (he₁ : e₁.is_affine) (he₂ : e₂.is_affine) (x : ℕ) :
---     ∀ y, (e₁.substₑ x e₂).count y ≤ 1 := by
---   intro y
---   match e₁ with
---   | .var x' =>
---     have : count (var x') y ≤ 1 := by simp only [count, ite_le_one (le_refl 1) (zero_le 1)]
---     simp_rw [substₑ, apply_ite (count · y), ite_le_one (affine_count_le_one he₂ y) this]
-
---   | .app a₁ a₂ =>
---     have ⟨ha₁, ha₂, hc⟩ := he₁
---     simp only [substₑ, count]
---     sorry
-
---   | .abs x e => sorry
-
-theorem affine_substₑ_is_affine {e₁ e₂ : Lambda} (he₁ : e₁.is_affine) (he₂ : e₂.is_affine) (x : ℕ) :
-    (e₁.substₑ x e₂).is_affine := by
-  unfold substₑ
-  match e₁ with
-  | .var x' => simp only [apply_ite, he₂, he₁, ite_self]
-  | .app a₁ a₂ =>
-    have ⟨ha₁, ha₂, hc⟩ := is_affine_of_app.mp he₁
-    simp only [is_affine, affine_substₑ_is_affine ha₁ he₂, affine_substₑ_is_affine ha₂ he₂,
-      true_and, decide_eq_true_eq]
-    intro x hx
-
-
-  | .abs x' e₁ => sorry
-
 def small_step (e : Lambda) : Lambda :=
   match e with
+  | .var x => .var x
+  | .abs x e => .abs x e.small_step
+  | .app (.var x) e₂ => .app (.var x) e₂.small_step
   | .app (.abs x e₁) e₂ => e₁.substₑ x e₂
-  | e => e
+  | .app (.app e₁ e₂) e₃ => .app (.app e₁.small_step e₂.small_step) e₃.small_step
 
-theorem small_step_is_affine {e : Lambda} (he : e.is_affine) : (e.small_step.is_affine) := by
+theorem small_step_count_β_lt (e : Lambda) (h : e.count_β ≠ 0) : e.small_step.count_β < e.count_β := by
   match e with
-  | .var _ => simp only [small_step, is_affine]
-  | .abs x e => simp only [small_step, is_affine, and_self, is_affine_of_abs.mp he, decide_True]
+  | .var x => simp only [count_β, ne_eq, not_true_eq_false] at h
+  | .abs x e => simp only [count_β, small_step_count_β_lt e h]
+  | .app (.var x) e₂ => sorry
+  | .app (.abs x e₁) e₂ => sorry
+  | .app (.app e₁ e₂) e₃ => sorry
 
-  | .app (.abs x e₁) e₂ =>
-    have ⟨he₁, he₂, _⟩ := is_affine_of_app.mp he
-    simp only [small_step, substₑ, is_affine, affine_substₑ_is_affine he₁ he₂]
+def normalize (e : Lambda) : Lambda :=
+  if h : e.count_β = 0 then
+    e
+  else
+    have : e.small_step.count_β < e.count_β := e.small_step_count_β_lt h
+    e.small_step.normalize
+
+termination_by e.count_β
+
+@[simp] theorem small_step_count (e : Lambda) (x : ℕ) : e.small_step.count x = e.count x := by sorry
+@[simp] theorem small_step_free (e : Lambda) : e.small_step.free = e.free := by sorry
+
+@[simp] theorem small_step_is_affine {e : Lambda} (h : e.is_affine) : e.small_step.is_affine := by
+  match e with
+  | .var x => simp only [small_step, h]
+
+  | .abs x e =>
+    have ⟨he, hc⟩ := is_affine_of_abs.mp h
+    simp only [small_step, small_step_is_affine he, is_affine_of_abs, small_step_count e x, hc,
+      and_self]
 
   | .app (.var x) e₂ =>
-    have ⟨_, he₂, hc⟩ := he
-    simp only [small_step, is_affine, he₂, hc, true_and, forall_const]
+    simp only [is_affine_of_app, is_affine_of_var, true_and] at h
+    have ⟨he₂, hinter⟩ := h
+    simp only [small_step, is_affine_of_app, is_affine_of_var, small_step_is_affine he₂, hinter,
+      small_step_free, true_and]
+
+  | .app (.abs x e₁) e₂ =>
+    simp only [is_affine_of_app, is_affine_of_abs] at h
+    have ⟨⟨he₁, _⟩, he₂, _⟩ := h
+    simp only [small_step, is_affine_substₑ he₁ he₂]
 
   | .app (.app e₁ e₂) e₃ =>
-    have ⟨⟨he₁, he₂, hc⟩, he₃, hc'⟩ := he
-    simp only [small_step, is_affine, he₁, he₂, he₃, hc, hc', true_and, forall_const]
+    simp only [is_affine_of_app, free] at h
+    have ⟨⟨he₁, he₂, hfree₁₂⟩, he₃, hfree₁₂₃⟩ := h
+    simp only [small_step, is_affine_of_app, small_step_is_affine he₁, small_step_is_affine he₂,
+      small_step_is_affine he₃, small_step_free, free, hfree₁₂, hfree₁₂₃, true_and]
 
-theorem small_step_free_subset (e : Lambda) : e.small_step.free ⊆ e.free := by
-  match e with
-  | .var x
-  | .abs x e
-  | .app (.var x) e₂
-  | .app (.app e₁ e₂) e₃
-  | .app (.abs x e₁) e₂ => simp only [free, small_step, substₑ_free_eq, Finset.Subset.refl]
+@[simp] theorem normalize_of_var (x : ℕ) : (var x).normalize = var x := by
+  unfold normalize
+  simp only [count_β, dif_pos]
+
+@[simp] theorem normalize_of_abs (e : Lambda) (x : ℕ) : (abs x e).normalize = abs x e.normalize := by
+  unfold normalize
+  simp only [count_β, dif_pos]
+  by_cases hc : e.count_β = 0
+  · simp_rw [dif_pos hc]
+  · have : e.small_step.count_β < e.count_β := small_step_count_β_lt e hc
+    simp_rw [dif_neg hc, small_step, normalize_of_abs e.small_step]
+termination_by e.count_β
+
+@[simp] theorem normalize_free_eq (e : Lambda) : e.normalize.free = e.free := by
+  unfold normalize
+  simp only [count_β, dif_pos]
+  by_cases hc : e.count_β = 0
+  · simp_rw [dif_pos hc]
+  · have : e.small_step.count_β < e.count_β := small_step_count_β_lt e hc
+    simp_rw [dif_neg hc, normalize_free_eq e.small_step, small_step_free]
+termination_by e.count_β
+
+@[simp] theorem normalize_affine {e : Lambda} (h : e.is_affine) : e.normalize.is_affine := by
+  if hβ : e.count_β = 0 then
+    rw [normalize, dif_pos hβ]
+    exact h
+  else
+    rw [normalize, dif_neg hβ]
+    simp only
+    have : e.small_step.count_β < e.count_β := small_step_count_β_lt e hβ
+    exact normalize_affine (small_step_is_affine h)
+termination_by e.count_β
 
 end Lambda
 
 namespace Affine
 
-def small_step (e : Affine vs) : (vs' : Finset ℕ) × (e : Affine vs') ×' (vs' ⊆ vs) := by
-  let el := e.to_lambda.small_step
-  let hel : el.is_affine := Lambda.small_step_is_affine (to_lambda_is_affine e)
-  let ⟨vs', e', he'⟩ := Affine.of_lambda_impl el hel
-  have hvs : vs = e.to_lambda.free := by sorry
-  have hvs' : vs' = el.free := by sorry
-  have hsub : el.free ⊆ e.to_lambda.free := Lambda.small_step_free_subset e.to_lambda
+def normalize (e : Affine vs) : (vs' : Finset ℕ) × (_ : Affine vs') ×' (vs' = vs) :=
+  let e' := e.to_lambda.normalize
 
-  refine' ⟨vs', e', _⟩
-  simp_rw [hvs', hvs, hsub]
+  have he'_free_sub : e'.free = vs := by
+    rw [e.free_eq, to_lambda_free_eq e]
+    exact Lambda.normalize_free_eq e.to_lambda
 
-#eval (Lambda.abs 2 (.var 1)).free
-#eval (Lambda.app (.abs 1 (.abs 2 (.var 1))) (.var 2)).small_step
-#eval (Affine.app (.abs 1 (.abs 2 (.var 1))) (.var 2) (by simp)).small_step.2.1
+  have he'_is_affine : e'.is_affine := Lambda.normalize_affine e.to_lambda_is_affine
 
-/-
-  TODO:
-  - small_step reduces number of abstractions
-  - todo normalize : repeatedly apply small step
--/
+  ⟨e'.free, Affine.of_lambda he'_is_affine, he'_free_sub⟩
 
 end Affine
