Affine/Affine.lean
@@ -40,15 +40,6 @@ def count (e : Affine vs) (x : ℕ) : ℕ :=
   | .abs x' e => if x = x' then 0 else count e x
   | .app e₁ e₂ _ => count e₁ x + count e₂ x
 
-/-- Number of β-reductions. That is, `(λ x. e₁) e₂`. -/
-def count_β (e : Affine vs) : ℕ :=
-  match e with
-  | .var x => 0
-  | .abs _ e => e.count_β
-  | .app (.var _) e₂ _ => e₂.count_β
-  | .app (.abs _ e₁) e₂ _ => 1 + e₁.count_β + e₂.count_β
-  | .app (.app e₁ e₂ _) e₃ _ => e₁.count_β + e₂.count_β + e₃.count_β
-
 /-- Whether all variables occur at most once. -/
 def is_affine (e : Affine vs) : Bool :=
   match e with
