Affine/Substitution.lean
@@ -1,0 +1,38 @@
+import «Affine».Lemmas
+
+namespace Lambda
+
+/-- Replaces free occurrences of variable `x` with variable `y`. -/
+def substᵥ (e : Lambda) (x y : ℕ) : Lambda :=
+  match e with
+  | .var x' => if x = x' then .var y else .var x'
+  | .app e₁ e₂ => .app (e₁.substᵥ x y) (e₂.substᵥ x y)
+  | .abs x' e => if x = x' then .abs x' e else .abs x' (e.substᵥ x y)
+
+/-- Variable substitution preserves depth. Needed for `termination_by` in `substₑ`. -/
+@[simp] theorem substᵥ_depth_eq (e : Lambda) (x y : ℕ) : (e.substᵥ x y).depth = e.depth := by
+  match e with
+  | .var x' => simp only [substᵥ, depth, apply_ite, ite_self]
+  | .app e₁ e₂ => simp only [substᵥ, depth, substᵥ_depth_eq]
+  | .abs x' e => simp only [substᵥ, apply_ite, depth, substᵥ_depth_eq, ite_self]
+
+/-- Substitutes free occurrences of variable `x` in `e₁` with `e₂`. -/
+def substₑ (e₁ : Lambda) (x : ℕ) (e₂ : Lambda) : Lambda :=
+  match e₁ with
+  | .var x' => if x = x' then e₂ else e₁
+  | .app a₁ a₂ => .app (a₁.substₑ x e₂) (a₂.substₑ x e₂)
+  | .abs x' e₁ =>
+    if x = x' ∨ x ∉ e₁.free then
+      .abs x' e₁
+    else if x' ∈ e₂.free then
+      let y := e₂.free.fresh
+      .abs y ((e₁.substᵥ x' y).substₑ x e₂)
+    else
+      .abs x' (e₁.substₑ x e₂)
+termination_by e₁.depth
+
+theorem is_affine_substₑ {e₁ e₂ : Lambda} (he₁ : e₁.is_affine) (he₂ : e₂.is_affine) (x : ℕ) :
+    (e₁.substₑ x e₂).is_affine := by
+  sorry
+
+end Lambda
